Prove lemma factorize_preserves_resolvability

Simple_Clause_Learning/Correct_Termination.thy
@@ -216,23 +216,6 @@ next
     by (cases u) (auto simp add: trail_minimal_subst_domains_def)
 qed
 
-definition trail_groundings where
-  "trail_groundings \<Gamma> \<longleftrightarrow> (\<forall>(_, n) \<in> set \<Gamma>.
-    case n of
-      None \<Rightarrow> True
-    | Some (C, L, \<gamma>) \<Rightarrow> is_ground_cls (add_mset L C \<cdot> \<gamma>))"
-
-lemma trail_groundings_if_sound: "sound_trail N \<Gamma> \<Longrightarrow> trail_groundings \<Gamma>"
-proof (induction \<Gamma> rule: sound_trail.induct)
-  case Nil
-  then show ?case
-    by (simp add: trail_groundings_def)
-next
-  case (Cons \<Gamma> L u)
-  then show ?case
-    by (cases u) (auto simp add: trail_groundings_def)
-qed
-
 theorem correct_termination:
   fixes gnd_N and gnd_N_lt_\<beta>
   assumes
